Test/comp/UnicodeStrings.dfy
@@ -5,11 +5,29 @@
 newtype uint32 = x: int | 0 <= x < 0x1_0000_0000
 newtype int32 = x: int | -0x8000_0000 <= x < 0x8000_0000
 
+// WARNING: Do not do this in real code!
+// It's a great example of what NOT to do when working with Unicode,
+// since the concept of upper/lower case is culture-specific.
+function method toLower(ch: char): char {
+  if 'A' <= ch <= 'Z' then
+    ch - 'A' + 'a'
+  else
+    ch
+}
+
 method Main(args: seq<string>) {
   var trickyString := "Dafny is just so " + [0x1F60E as char];
   print trickyString, "\n";
 
+  // Testing that runtimes don't confuse a seq<uint32> for a string
+  // (which would be a problem if we used Int32 in C# instead of Rune, for example)
   var s := "Ceci n'est pas une string";
   var notAString := seq(|s|, i requires 0 <= i < |s| => s[i] as int32);
   print notAString, "\n";
+
+  var sarcastic := "Oh UNicOdE, tHaT's a REaL usEFuL FEaTuRe!";
+  var sincere := seq(|sarcastic|, i requires 0 <= i < |sarcastic| => toLower(sarcastic[i]));
+  print sincere, "\n";
 }
+
+
